Parametrization

src/syntax/FStar.Syntax.Print.fst
@@ -42,23 +42,23 @@ let rec delta_depth_to_string = function
     | Delta_equational_at_level i -> "Delta_equational_at_level " ^ string_of_int i
     | Delta_abstract d -> "Delta_abstract (" ^ delta_depth_to_string d ^ ")"
 
-let sli (l:lident) : string =
-    if Options.print_real_names()
+let sli opts (l:lident) : string =
+    if opts.print_real_names
     then string_of_lid l
     else string_of_id (ident_of_lid l)
 //    Util.format3 "%s@{def=%s;use=%s}" s
 //        (Range.string_of_range (Ident.range_of_lid l))
 //        (Range.string_of_use_range (Ident.range_of_lid l))
 
-let lid_to_string (l:lid) = sli l
+let lid_to_string opts (l:lid) = sli opts l
 
-// let fv_to_string fv = Printf.sprintf "%s@%A" (lid_to_string fv.fv_name.v) fv.fv_delta
-let fv_to_string fv = lid_to_string fv.fv_name.v //^ "(@@" ^ delta_depth_to_string fv.fv_delta ^ ")"
-let bv_to_string bv = (string_of_id bv.ppname) ^ "#" ^ (string_of_int bv.index)
+// let fv_to_string opts fv = Printf.sprintf "%s@%A" (lid_to_string opts opts fv.fv_name.v) fv.fv_delta
+let fv_to_string opts fv = lid_to_string opts fv.fv_name.v //^ "(@@" ^ delta_depth_to_string fv.fv_delta ^ ")"
+let bv_to_string opts bv = (string_of_id bv.ppname) ^ "#" ^ (string_of_int bv.index)
 
-let nm_to_string bv =
-    if Options.print_real_names()
-    then bv_to_string bv
+let nm_to_string opts bv =
+    if opts.print_real_names
+    then bv_to_string opts bv
     else (string_of_id bv.ppname)
 
 let db_to_string bv = (string_of_id bv.ppname) ^ "@" ^ string_of_int bv.index
@@ -141,14 +141,14 @@ let quant_to_string t = find_lid (get_lid t) quants
 
 let const_to_string x = C.const_to_string x
 
-let lbname_to_string = function
-  | Inl l -> bv_to_string l
-  | Inr l -> lid_to_string l.fv_name.v
+let lbname_to_string opts = function
+  | Inl l -> bv_to_string opts l
+  | Inr l -> lid_to_string opts l.fv_name.v
 
-let uvar_to_string u = if (Options.hide_uvar_nums()) then "?" else "?" ^ (Unionfind.uvar_id u |> string_of_int)
+let uvar_to_string opts u = if opts.hide_uvar_nums then "?" else "?" ^ (Unionfind.uvar_id u |> string_of_int)
 let version_to_string v = U.format2 "%s.%s" (U.string_of_int v.major) (U.string_of_int v.minor)
-let univ_uvar_to_string u =
-    if (Options.hide_uvar_nums())
+let univ_uvar_to_string opts u =
+    if opts.hide_uvar_nums
     then "?"
     else "?" ^ (Unionfind.univ_uvar_id u |> string_of_int)
             ^ ":" ^ (u |> (fun (_, u, _) -> version_to_string u))
@@ -158,33 +158,33 @@ let rec int_of_univ n u = match Subst.compress_univ u with
     | U_succ u -> int_of_univ (n+1) u
     | _ -> n, Some u
 
-let rec univ_to_string u =
+let rec univ_to_string opts u =
 Errors.with_ctx "While printing universe" (fun () ->
   // VD: commented out for testing NBE
-  // if not (Options.ugly()) then
+  // if not (opts.ugly()) then
   //   let e = Resugar.resugar_universe u Range.dummyRange in
   //   let d = ToDocument.term_to_document e in
   //   Pp.pretty_string (float_of_string "1.0") 100 d
   // else
   match Subst.compress_univ u with
-    | U_unif u -> "U_unif "^univ_uvar_to_string u
+    | U_unif u -> "U_unif "^univ_uvar_to_string opts u
     | U_name x -> "U_name "^(string_of_id x)
     | U_bvar x -> "@"^string_of_int x
     | U_zero   -> "0"
     | U_succ u ->
         begin match int_of_univ 1 u with
             | n, None -> string_of_int n
-            | n, Some u -> U.format2 "(%s + %s)" (univ_to_string u) (string_of_int n)
+            | n, Some u -> U.format2 "(%s + %s)" (univ_to_string opts u) (string_of_int n)
         end
-    | U_max us -> U.format1 "(max %s)" (List.map univ_to_string us |> String.concat ", ")
+    | U_max us -> U.format1 "(max %s)" (List.map (univ_to_string opts) us |> String.concat ", ")
     | U_unknown -> "unknown"
 )
 
-let univs_to_string us = List.map univ_to_string us |> String.concat ", "
+let univs_to_string opts us = List.map (univ_to_string opts) us |> String.concat ", "
 
 let univ_names_to_string us = List.map (fun x -> (string_of_id x)) us |> String.concat ", "
 
-let qual_to_string = function
+let qual_to_string opts = function
   | Assumption            -> "assume"
   | New                   -> "new"
   | Private               -> "private"
@@ -197,11 +197,11 @@ let qual_to_string = function
   | Unopteq               -> "unopteq"
   | Logic                 -> "logic"
   | TotalEffect           -> "total"
-  | Discriminator l       -> U.format1 "(Discriminator %s)" (lid_to_string l)
-  | Projector (l, x)      -> U.format2 "(Projector %s %s)" (lid_to_string l) (string_of_id x)
+  | Discriminator l       -> U.format1 "(Discriminator %s)" (lid_to_string opts l)
+  | Projector (l, x)      -> U.format2 "(Projector %s %s)" (lid_to_string opts l) (string_of_id x)
   | RecordType (ns, fns)  -> U.format2 "(RecordType %s %s)" (text_of_path (path_of_ns ns)) (fns |> List.map string_of_id |> String.concat ", ")
   | RecordConstructor (ns, fns) -> U.format2 "(RecordConstructor %s %s)" (text_of_path (path_of_ns ns))  (fns |> List.map string_of_id |> String.concat ", ")
-  | Action eff_lid        -> U.format1 "(Action %s)" (lid_to_string eff_lid)
+  | Action eff_lid        -> U.format1 "(Action %s)" (lid_to_string opts eff_lid)
   | ExceptionConstructor  -> "ExceptionConstructor"
   | HasMaskedEffect       -> "HasMaskedEffect"
   | Effect                -> "Effect"
@@ -209,15 +209,15 @@ let qual_to_string = function
   | Reflectable l         -> U.format1 "(reflect %s)" (string_of_lid l)
   | OnlyName              -> "OnlyName"
 
-let quals_to_string quals =
+let quals_to_string opts quals =
     match quals with
     | [] -> ""
-    | _ -> quals |> List.map qual_to_string |> String.concat " "
+    | _ -> quals |> List.map (qual_to_string opts) |> String.concat " "
 
-let quals_to_string' quals =
+let quals_to_string' opts quals =
     match quals with
     | [] -> ""
-    | _ -> quals_to_string quals ^ " "
+    | _ -> quals_to_string opts quals ^ " "
 
 
 let paren s = "(" ^ s ^ ")"
@@ -227,10 +227,10 @@ let paren s = "(" ^ s ^ ")"
    function in normalize.fs instead, since elaboration
    (higher-order unification) produces types containing lots of
    redexes that should first be reduced. *)
-let rec tag_of_term (t:term) = match t.n with
+let rec tag_of_term opts (t:term) = match t.n with
   | Tm_bvar x -> "Tm_bvar: "   ^ db_to_string x
-  | Tm_name x -> "Tm_name: " ^ nm_to_string x
-  | Tm_fvar x -> "Tm_fvar: "   ^ lid_to_string x.fv_name.v
+  | Tm_name x -> "Tm_name: " ^ nm_to_string opts x
+  | Tm_fvar x -> "Tm_fvar: "   ^ lid_to_string opts x.fv_name.v
   | Tm_uinst _ -> "Tm_uinst"
   | Tm_constant _ -> "Tm_constant"
   | Tm_type _ -> "Tm_type"
@@ -245,19 +245,19 @@ let rec tag_of_term (t:term) = match t.n with
   | Tm_let _ -> "Tm_let"
   | Tm_uvar _ -> "Tm_uvar"
   | Tm_delayed _ -> "Tm_delayed"
-  | Tm_meta (_, m) -> "Tm_meta:" ^ metadata_to_string m
+  | Tm_meta (_, m) -> "Tm_meta:" ^ metadata_to_string opts m
   | Tm_unknown -> "Tm_unknown"
   | Tm_lazy _ -> "Tm_lazy"
 
-and term_to_string x =
-  if not (Options.ugly()) then
+and term_to_string opts x =
+  if not opts.ugly then
     let e = Errors.with_ctx "While resugaring a term" (fun () -> Resugar.resugar_term x) in
     let d = ToDocument.term_to_document e in
     Pp.pretty_string (float_of_string "1.0") 100 d
   else begin
     Errors.with_ctx "While ugly-printing a term" (fun () ->
       let x = Subst.compress x in
-      let x = if Options.print_implicits() then x else SU.unmeta x in
+      let x = if opts.print_implicits then x else SU.unmeta x in
       match x.n with
       | Tm_delayed _ ->   failwith "impossible"
       | Tm_app(_, []) ->  failwith "Empty args!"
@@ -265,119 +265,119 @@ and term_to_string x =
       // TODO: add an option to mark where this happens
       | Tm_lazy ({blob=b; lkind=Lazy_embedding (_, thunk)}) ->
         "[LAZYEMB:" ^
-        term_to_string (Thunk.force thunk) ^ "]"
+        term_to_string opts (Thunk.force thunk) ^ "]"
       | Tm_lazy i ->
         "[lazy:" ^
-        term_to_string (must !lazy_chooser i.lkind i) // can't call into Syntax.Util here..
+        term_to_string opts (must !lazy_chooser i.lkind i) // can't call into Syntax.Util here..
         ^"]"
 
       | Tm_quoted (tm, qi) ->
         begin match qi.qkind with
         | Quote_static ->
             let print_aq (bv, t) =
-              U.format2 "%s -> %s" (bv_to_string bv) (term_to_string t)
+              U.format2 "%s -> %s" (bv_to_string opts bv) (term_to_string opts t)
             in
-            U.format2 "`(%s)%s" (term_to_string tm)
+            U.format2 "`(%s)%s" (term_to_string opts tm)
                                 (FStar.Common.string_of_list print_aq qi.antiquotes)
         | Quote_dynamic ->
-            U.format1 "quote (%s)" (term_to_string tm)
+            U.format1 "quote (%s)" (term_to_string opts tm)
         end
 
       | Tm_meta(t, Meta_pattern (_, ps)) ->
-        let pats = ps |> List.map (fun args -> args |> List.map (fun (t, _) -> term_to_string t) |> String.concat "; ") |> String.concat "\/" in
-        U.format2 "{:pattern %s} %s" pats (term_to_string t)
+        let pats = ps |> List.map (fun args -> args |> List.map (fun (t, _) -> term_to_string opts t) |> String.concat "; ") |> String.concat "\/" in
+        U.format2 "{:pattern %s} %s" pats (term_to_string opts t)
 
-      | Tm_meta(t, Meta_monadic (m, t')) -> U.format4 ("(MetaMonadic-{%s %s} (%s) %s)") (sli m) (term_to_string t') (tag_of_term t) (term_to_string t)
+      | Tm_meta(t, Meta_monadic (m, t')) -> U.format4 ("(MetaMonadic-{%s %s} (%s) %s)") (sli opts m) (term_to_string opts t') (tag_of_term opts t) (term_to_string opts t)
 
-      | Tm_meta(t, Meta_monadic_lift(m0, m1, t')) -> U.format4 ("(MetaMonadicLift-{%s : %s -> %s} %s)") (term_to_string t') (sli m0) (sli m1) (term_to_string t)
+      | Tm_meta(t, Meta_monadic_lift(m0, m1, t')) -> U.format4 ("(MetaMonadicLift-{%s : %s -> %s} %s)") (term_to_string opts t') (sli opts m0) (sli opts m1) (term_to_string opts t)
 
       | Tm_meta(t, Meta_labeled(l,r,b)) ->
-        U.format3 "Meta_labeled(%s, %s){%s}" l (Range.string_of_range r) (term_to_string t)
+        U.format3 "Meta_labeled(%s, %s){%s}" l (Range.string_of_range r) (term_to_string opts t)
 
       | Tm_meta(t, Meta_named(l)) ->
-        U.format3 "Meta_named(%s, %s){%s}" (lid_to_string l) (Range.string_of_range t.pos) (term_to_string t)
+        U.format3 "Meta_named(%s, %s){%s}" (lid_to_string opts l) (Range.string_of_range t.pos) (term_to_string opts t)
 
       | Tm_meta(t, Meta_desugared _) ->
-        U.format1 "Meta_desugared{%s}"  (term_to_string t)
+        U.format1 "Meta_desugared{%s}"  (term_to_string opts t)
 
-      | Tm_bvar x ->        db_to_string x ^ ":(" ^ (tag_of_term x.sort) ^  ")"
-      | Tm_name x ->        nm_to_string x // ^ "@@(" ^ term_to_string x.sort ^ ")"
-      | Tm_fvar f ->        fv_to_string f
+      | Tm_bvar x ->        db_to_string x ^ ":(" ^ (tag_of_term opts x.sort) ^  ")"
+      | Tm_name x ->        nm_to_string opts x // ^ "@@(" ^ term_to_string opts x.sort ^ ")"
+      | Tm_fvar f ->        fv_to_string opts f
       | Tm_uvar (u, ([], _)) ->
-        if Options.print_bound_var_types()
-        && Options.print_effect_args()
-        then ctx_uvar_to_string_aux true u
+        if opts.print_bound_var_types
+        && opts.print_effect_args
+        then ctx_uvar_to_string_aux opts true u
         else "?" ^ (string_of_int <| Unionfind.uvar_id u.ctx_uvar_head)
       | Tm_uvar (u, s) ->
-        if Options.print_bound_var_types()
-        && Options.print_effect_args()
-        then U.format2 "(%s @ %s)" (ctx_uvar_to_string_aux true u) (List.map subst_to_string (fst s) |> String.concat "; ")
+        if opts.print_bound_var_types
+        && opts.print_effect_args
+        then U.format2 "(%s @ %s)" (ctx_uvar_to_string_aux opts true u) (List.map (subst_to_string opts) (fst s) |> String.concat "; ")
         else "?" ^ (string_of_int <| Unionfind.uvar_id u.ctx_uvar_head)
       | Tm_constant c ->    const_to_string c
-      | Tm_type u ->        if (Options.print_universes()) then U.format1 "Type u#(%s)" (univ_to_string u) else "Type"
-      | Tm_arrow(bs, c) ->  U.format2 "(%s -> %s)"  (binders_to_string " -> " bs) (comp_to_string c)
+      | Tm_type u ->        if opts.print_universes then U.format1 "Type u#(%s)" (univ_to_string opts u) else "Type"
+      | Tm_arrow(bs, c) ->  U.format2 "(%s -> %s)"  (binders_to_string opts " -> " bs) (comp_to_string opts c)
       | Tm_abs(bs, t2, lc) ->
         begin match lc with
-            | Some rc when (Options.print_implicits()) ->
+            | Some rc when opts.print_implicits ->
               U.format4 "(fun %s -> (%s $$ (residual) %s %s))"
-                            (binders_to_string " " bs)
-                            (term_to_string t2)
+                            (binders_to_string opts " " bs)
+                            (term_to_string opts t2)
                             (string_of_lid rc.residual_effect)
-                            (if Option.isNone rc.residual_typ then "None" else term_to_string (Option.get rc.residual_typ))
+                            (if Option.isNone rc.residual_typ then "None" else term_to_string opts (Option.get rc.residual_typ))
             | _ ->
-              U.format2 "(fun %s -> %s)" (binders_to_string " " bs) (term_to_string t2)
+              U.format2 "(fun %s -> %s)" (binders_to_string opts " " bs) (term_to_string opts t2)
         end
-      | Tm_refine(xt, f) -> U.format3 "(%s:%s{%s})" (bv_to_string xt) (xt.sort |> term_to_string) (f |> formula_to_string)
-      | Tm_app(t, args) ->  U.format2 "(%s %s)" (term_to_string t) (args_to_string args)
-      | Tm_let(lbs, e) ->   U.format2 "%s\nin\n%s" (lbs_to_string [] lbs) (term_to_string e)
+      | Tm_refine(xt, f) -> U.format3 "(%s:%s{%s})" (bv_to_string opts xt) (xt.sort |> term_to_string opts) (f |> formula_to_string opts)
+      | Tm_app(t, args) ->  U.format2 "(%s %s)" (term_to_string opts t) (args_to_string opts args)
+      | Tm_let(lbs, e) ->   U.format2 "%s\nin\n%s" (lbs_to_string opts [] lbs) (term_to_string opts e)
       | Tm_ascribed(e,(annot, topt, b),eff_name) ->
         let annot = match annot with
-            | Inl t -> U.format2 "[%s] %s" (map_opt eff_name Ident.string_of_lid |> dflt "default") (term_to_string t)
-            | Inr c -> comp_to_string c in
+            | Inl t -> U.format2 "[%s] %s" (map_opt eff_name Ident.string_of_lid |> dflt "default") (term_to_string opts t)
+            | Inr c -> comp_to_string opts c in
         let topt = match topt with
             | None -> ""
-            | Some t -> U.format1 "by %s" (term_to_string t) in
+            | Some t -> U.format1 "by %s" (term_to_string opts t) in
         let s = if b then "ascribed_eq" else "ascribed" in
-        U.format4 "(%s <%s: %s %s)" (term_to_string e) s annot topt
+        U.format4 "(%s <%s: %s %s)" (term_to_string opts e) s annot topt
       | Tm_match(head, asc_opt, branches, lc) ->
         let lc_str =
           match lc with
-          | Some lc when (Options.print_implicits ()) ->
+          | Some lc when opts.print_implicits ->
             U.format1 " (residual_comp:%s)"
-              (if Option.isNone lc.residual_typ then "None" else term_to_string (Option.get lc.residual_typ))
+              (if Option.isNone lc.residual_typ then "None" else term_to_string opts (Option.get lc.residual_typ))
           | _ -> "" in
         U.format4 "(match %s %swith\n\t| %s%s)"
-          (term_to_string head)
+          (term_to_string opts head)
           (match asc_opt with
            | None -> ""
            | Some (b, (asc, tacopt, use_eq)) ->
              let s = if use_eq then "returns$" else "returns" in
              U.format4 "as %s %s %s%s "
-               (binder_to_string b)
+               (binder_to_string opts b)
                s
                (match asc with
-                | Inl t -> term_to_string t
-                | Inr c -> comp_to_string c)
+                | Inl t -> term_to_string opts t
+                | Inr c -> comp_to_string opts c)
                (match tacopt with
                 | None -> ""
-                | Some tac -> U.format1 " by %s" (term_to_string tac)))
-          (U.concat_l "\n\t|" (branches |> List.map branch_to_string))
+                | Some tac -> U.format1 " by %s" (term_to_string opts tac)))
+          (U.concat_l "\n\t|" (branches |> List.map (branch_to_string opts)))
           lc_str
       | Tm_uinst(t, us) ->
-        if (Options.print_universes())
-        then U.format2 "%s<%s>" (term_to_string t) (univs_to_string us)
-        else term_to_string t
+        if opts.print_universes
+        then U.format2 "%s<%s>" (term_to_string opts t) (univs_to_string opts us)
+        else term_to_string opts t
 
       | Tm_unknown -> "_"
     )
   end
 
-and branch_to_string (p, wopt, e) : string =
+and branch_to_string opts (p, wopt, e) : string =
     U.format3 "%s %s -> %s"
-                (p |> pat_to_string)
-                (match wopt with | None -> "" | Some w -> U.format1 "when %s" (w |> term_to_string))
-                (e |> term_to_string)
-and ctx_uvar_to_string_aux print_reason ctx_uvar =
+                (p |> pat_to_string opts)
+                (match wopt with | None -> "" | Some w -> U.format1 "when %s" (w |> term_to_string opts))
+                (e |> term_to_string opts)
+and ctx_uvar_to_string_aux opts print_reason ctx_uvar =
     let reason_string =
       if print_reason
       then U.format1 "(* %s *)\n" ctx_uvar.ctx_uvar_reason
@@ -386,44 +386,44 @@ and ctx_uvar_to_string_aux print_reason ctx_uvar =
              (Range.string_of_pos (Range.end_of_range ctx_uvar.ctx_uvar_range)) in
     format4 "%s(%s |- %s : %s)"
             reason_string
-            (binders_to_string ", " ctx_uvar.ctx_uvar_binders)
-            (uvar_to_string ctx_uvar.ctx_uvar_head)
-            (term_to_string ctx_uvar.ctx_uvar_typ)
+            (binders_to_string opts ", " ctx_uvar.ctx_uvar_binders)
+            (uvar_to_string opts ctx_uvar.ctx_uvar_head)
+            (term_to_string opts ctx_uvar.ctx_uvar_typ)
 
-and subst_elt_to_string = function
-   | DB(i, x) -> U.format2 "DB (%s, %s)" (string_of_int i) (bv_to_string x)
-   | NM(x, i) -> U.format2 "NM (%s, %s)" (bv_to_string x) (string_of_int i)
-   | NT(x, t) -> U.format2 "NT (%s, %s)" (bv_to_string x) (term_to_string t)
-   | UN(i, u) -> U.format2 "UN (%s, %s)" (string_of_int i) (univ_to_string u)
+and subst_elt_to_string opts = function
+   | DB(i, x) -> U.format2 "DB (%s, %s)" (string_of_int i) (bv_to_string opts x)
+   | NM(x, i) -> U.format2 "NM (%s, %s)" (bv_to_string opts x) (string_of_int i)
+   | NT(x, t) -> U.format2 "NT (%s, %s)" (bv_to_string opts x) (term_to_string opts t)
+   | UN(i, u) -> U.format2 "UN (%s, %s)" (string_of_int i) (univ_to_string opts u)
    | UD(u, i) -> U.format2 "UD (%s, %s)" (string_of_id u) (string_of_int i)
 
-and subst_to_string s = s |> List.map subst_elt_to_string |> String.concat "; "
+and subst_to_string opts s = s |> List.map (subst_elt_to_string opts) |> String.concat "; "
 
-and pat_to_string x =
-  if not (Options.ugly()) then
+and pat_to_string opts x =
+  if not opts.ugly then
     let e = Resugar.resugar_pat x (new_bv_set ()) in
     let d = ToDocument.pat_to_document e in
     Pp.pretty_string (float_of_string "1.0") 100 d
   else match x.v with
-    | Pat_cons(l, pats) -> U.format2 "(%s %s)" (fv_to_string l) (List.map (fun (x, b) -> let p = pat_to_string x in if b then "#"^p else p) pats |> String.concat " ")
+    | Pat_cons(l, pats) -> U.format2 "(%s %s)" (fv_to_string opts l) (List.map (fun (x, b) -> let p = pat_to_string opts x in if b then "#"^p else p) pats |> String.concat " ")
     | Pat_dot_term (x, _) ->
-      if Options.print_bound_var_types()
-      then U.format2 ".%s:%s" (bv_to_string x) (term_to_string x.sort)
-      else U.format1 ".%s" (bv_to_string x)
+      if opts.print_bound_var_types
+      then U.format2 ".%s:%s" (bv_to_string opts x) (term_to_string opts x.sort)
+      else U.format1 ".%s" (bv_to_string opts x)
     | Pat_var x ->
-      if Options.print_bound_var_types()
-      then U.format2 "%s:%s" (bv_to_string x) (term_to_string x.sort)
-      else bv_to_string x
+      if opts.print_bound_var_types
+      then U.format2 "%s:%s" (bv_to_string opts x) (term_to_string opts x.sort)
+      else bv_to_string opts x
     | Pat_constant c -> const_to_string c
     | Pat_wild x ->
-      if Options.print_bound_var_types()
-      then U.format2 "_wild_%s:%s" (bv_to_string x) (term_to_string x.sort)
-      else bv_to_string x
+      if opts.print_bound_var_types
+      then U.format2 "_wild_%s:%s" (bv_to_string opts x) (term_to_string opts x.sort)
+      else bv_to_string opts x
 
 
-and lbs_to_string quals lbs =
+and lbs_to_string opts quals lbs =
 //    let lbs =
-//        if (Options.print_universes())
+//        if (opts.print_universes())
 //        then (fst lbs, snd lbs |> List.map (fun lb -> let us, td = Subst.open_univ_vars lb.lbunivs (Util.mk_conj lb.lbtyp lb.lbdef) in
 //                                        let t, d = match (Subst.compress td).n with
 //                                            | Tm_app(_, [(t, _); (d, _)]) -> t, d
@@ -431,81 +431,81 @@ and lbs_to_string quals lbs =
 //                                        {lb with lbunivs=us; lbtyp=t; lbdef=d}))
 //        else lbs in
     U.format3 "%slet %s %s"
-    (quals_to_string' quals)
+    (quals_to_string' opts  quals)
     (if fst lbs then "rec" else "")
     (U.concat_l "\n and " (snd lbs |> List.map (fun lb ->
                                                     U.format5 "%s%s %s : %s = %s"
-                                                            (attrs_to_string lb.lbattrs)
-                                                            (lbname_to_string lb.lbname)
-                                                            (if (Options.print_universes())
+                                                            (attrs_to_string opts lb.lbattrs)
+                                                            (lbname_to_string opts lb.lbname)
+                                                            (if opts.print_universes
                                                              then "<"^univ_names_to_string lb.lbunivs^">"
                                                              else "")
-                                                            (term_to_string lb.lbtyp)
-                                                            (lb.lbdef |> term_to_string))))
-and attrs_to_string = function
+                                                            (term_to_string opts lb.lbtyp)
+                                                            (lb.lbdef |> term_to_string opts))))
+and attrs_to_string opts = function
     | [] -> ""
-    | tms -> U.format1 "[@ %s]" (List.map (fun t -> paren (term_to_string t)) tms |> String.concat "; ")
+    | tms -> U.format1 "[@ %s]" (List.map (fun t -> paren (term_to_string opts t)) tms |> String.concat "; ")
 
 //and uvar_t_to_string (uv, k) =
-//   if false && (Options.print_real_names())
+//   if false && (opts.print_real_names())
 //   then
 //       U.format2 "(U%s : %s)"
-//       (if (Options.hide_uvar_nums()) then "?" else U.string_of_int (Unionfind.uvar_id uv))
+//       (if (opts.hide_uvar_nums()) then "?" else U.string_of_int (Unionfind.uvar_id uv))
 //       (kind_to_string k)
-//   else U.format1 "U%s"  (if (Options.hide_uvar_nums()) then "?" else U.string_of_int (Unionfind.uvar_id uv))
+//   else U.format1 "U%s"  (if (opts.hide_uvar_nums()) then "?" else U.string_of_int (Unionfind.uvar_id uv))
 
-and bqual_to_string' s = function
+and bqual_to_string' opts s = function
   | Some (Implicit false) -> "#" ^ s
   | Some (Implicit true) -> "#." ^ s
   | Some Equality -> "$" ^ s
   | Some (Meta t) when SU.is_fvar C.tcresolve_lid t -> "{|" ^ s ^ "|}"
-  | Some (Meta t) -> "#[" ^ term_to_string t ^ "]" ^ s
+  | Some (Meta t) -> "#[" ^ term_to_string opts t ^ "]" ^ s
   | None -> s
 
 and aqual_to_string' s = function
   | Some ({aqual_implicit=true}) -> "#" ^ s
   | _ -> s
   
-and binder_to_string' is_arrow b =
-  if not (Options.ugly()) then
+and binder_to_string' opts is_arrow b =
+  if not opts.ugly then
     match Resugar.resugar_binder b Range.dummyRange with
     | None -> ""
     | Some e ->
       let d = ToDocument.binder_to_document e in
       Pp.pretty_string (float_of_string "1.0") 100 d
   else
-    let attrs = attrs_to_string b.binder_attrs in
+    let attrs = attrs_to_string opts b.binder_attrs in
     if is_null_binder b
-    then (attrs ^ "_:" ^ term_to_string b.binder_bv.sort)
-    else if not is_arrow && not (Options.print_bound_var_types())
-    then bqual_to_string' (attrs ^ nm_to_string b.binder_bv) b.binder_qual
-    else bqual_to_string' (attrs ^ nm_to_string b.binder_bv ^ ":" ^ term_to_string b.binder_bv.sort) b.binder_qual
+    then (attrs ^ "_:" ^ term_to_string opts b.binder_bv.sort)
+    else if not is_arrow && not opts.print_bound_var_types
+    then bqual_to_string' opts (attrs ^ nm_to_string opts b.binder_bv) b.binder_qual
+    else bqual_to_string' opts (attrs ^ nm_to_string opts b.binder_bv ^ ":" ^ term_to_string opts b.binder_bv.sort) b.binder_qual
 
-and binder_to_string b =  binder_to_string' false b
+and binder_to_string opts b =  binder_to_string' opts false b
 
-and arrow_binder_to_string b = binder_to_string' true b
+and arrow_binder_to_string opts b = binder_to_string' opts true b
 
-and binders_to_string sep bs =
+and binders_to_string opts sep bs =
     let bs =
-      if (Options.print_implicits())
+      if opts.print_implicits
       then bs
       else filter_imp_binders bs in
     if sep = " -> "
-    then bs |> List.map arrow_binder_to_string |> String.concat sep
-    else bs |> List.map binder_to_string |> String.concat sep
+    then bs |> List.map (arrow_binder_to_string opts) |> String.concat sep
+    else bs |> List.map (binder_to_string opts) |> String.concat sep
 
-and arg_to_string = function
-   | a,  imp -> aqual_to_string' (term_to_string a) imp
+and arg_to_string opts = function
+   | a,  imp -> aqual_to_string' (term_to_string opts a) imp
 
-and args_to_string args =
+and args_to_string opts args =
     let args =
-      if (Options.print_implicits())
+      if opts.print_implicits
       then args
       else filter_imp_args args in
-    args |> List.map arg_to_string |> String.concat " "
+    args |> List.map (arg_to_string opts) |> String.concat " "
 
-and comp_to_string c =
-  if not (Options.ugly()) then
+and comp_to_string opts c =
+  if not opts.ugly then
     let e = Errors.with_ctx "While resugaring a computation" (fun () -> Resugar.resugar_comp c) in
     let d = ToDocument.term_to_document e in
     Pp.pretty_string (float_of_string "1.0") 100 d
@@ -514,40 +514,40 @@ and comp_to_string c =
     match c.n with
     | Total (t, uopt) ->
       begin match (compress t).n with
-        | Tm_type _ when not (Options.print_implicits() || Options.print_universes()) -> term_to_string t
+        | Tm_type _ when not (opts.print_implicits || opts.print_universes) -> term_to_string opts t
         | _ ->
           match uopt with
-          | Some u when Options.print_universes() -> U.format2 "Tot<%s> %s" (univ_to_string u) (term_to_string t)
-          | _ -> U.format1 "Tot %s" (term_to_string t)
+          | Some u when opts.print_universes -> U.format2 "Tot<%s> %s" (univ_to_string opts u) (term_to_string opts t)
+          | _ -> U.format1 "Tot %s" (term_to_string opts t)
       end
     | GTotal (t, uopt) ->
       begin match (compress t).n with
-        | Tm_type _ when not (Options.print_implicits() || Options.print_universes()) -> term_to_string t
+        | Tm_type _ when not (opts.print_implicits || opts.print_universes) -> term_to_string opts t
         | _ ->
           match uopt with
-          | Some u when Options.print_universes() -> U.format2 "GTot<%s> %s" (univ_to_string u) (term_to_string t)
-          | _ -> U.format1 "GTot %s" (term_to_string t)
+          | Some u when opts.print_universes -> U.format2 "GTot<%s> %s" (univ_to_string opts u) (term_to_string opts t)
+          | _ -> U.format1 "GTot %s" (term_to_string opts t)
       end
     | Comp c ->
         let basic =
-          if (Options.print_effect_args())
+          if (opts.print_effect_args)
           then U.format5 "%s<%s> (%s) %s (attributes %s)"
-                            (sli c.effect_name)
-                            (c.comp_univs |> List.map univ_to_string |> String.concat ", ")
-                            (term_to_string c.result_typ)
-                            (c.effect_args |> List.map arg_to_string |> String.concat ", ")
-                            (cflags_to_string c.flags)
+                            (sli opts c.effect_name)
+                            (c.comp_univs |> List.map (univ_to_string opts) |> String.concat ", ")
+                            (term_to_string opts c.result_typ)
+                            (c.effect_args |> List.map (arg_to_string opts) |> String.concat ", ")
+                            (cflags_to_string opts c.flags)
           else if c.flags |> U.for_some (function TOTAL -> true | _ -> false)
-          && not (Options.print_effect_args())
-          then U.format1 "Tot %s" (term_to_string c.result_typ)
-          else if not (Options.print_effect_args())
-                  && not (Options.print_implicits())
+          && not opts.print_effect_args
+          then U.format1 "Tot %s" (term_to_string opts c.result_typ)
+          else if not opts.print_effect_args
+                  && not opts.print_implicits
                   && lid_equals c.effect_name (C.effect_ML_lid())
-          then term_to_string c.result_typ
-          else if not (Options.print_effect_args())
+          then term_to_string opts c.result_typ
+          else if not opts.print_effect_args
                && c.flags |> U.for_some (function MLEFFECT -> true | _ -> false)
-          then U.format1 "ALL %s" (term_to_string c.result_typ)
-          else U.format2 "%s (%s)" (sli c.effect_name) (term_to_string c.result_typ) in
+          then U.format1 "ALL %s" (term_to_string opts c.result_typ)
+          else U.format2 "%s (%s)" (sli opts c.effect_name) (term_to_string opts c.result_typ) in
       let dec = c.flags
         |> List.collect (function DECREASES dec_order ->
             (match dec_order with
@@ -557,16 +557,16 @@ and comp_to_string c =
                    | [] -> ""
                    | hd::tl ->
                      tl |> List.fold_left (fun s t ->
-                       s ^ ";" ^ term_to_string t) (term_to_string hd))]
+                       s ^ ";" ^ term_to_string opts t) (term_to_string opts hd))]
              | Decreases_wf (rel, e) ->
-               [U.format2 "(decreases {:well-founded %s %s})" (term_to_string rel) (term_to_string e)])
+               [U.format2 "(decreases {:well-founded %s %s})" (term_to_string opts rel) (term_to_string opts e)])
              | _ -> [])
             
         |> String.concat " " in
       U.format2 "%s%s" basic dec
     )
 
-and cflag_to_string c =
+and cflag_to_string opts c =
     match c with
         | TOTAL -> "total"
         | MLEFFECT -> "ml"
@@ -579,19 +579,19 @@ and cflag_to_string c =
         | CPS -> "cps"
         | DECREASES _ -> "" (* TODO : already printed for now *)
 
-and cflags_to_string fs = FStar.Common.string_of_list cflag_to_string fs
+and cflags_to_string opts fs = FStar.Common.string_of_list (cflag_to_string opts) fs
 
 (* CH: at this point not even trying to detect if something looks like a formula,
        only locally detecting certain patterns *)
-and formula_to_string phi = term_to_string phi
+and formula_to_string opts phi = term_to_string opts phi
 
-and metadata_to_string = function
+and metadata_to_string opts = function
     | Meta_pattern (_, ps) ->
-        let pats = ps |> List.map (fun args -> args |> List.map (fun (t, _) -> term_to_string t) |> String.concat "; ") |> String.concat "\/" in
+        let pats = ps |> List.map (fun args -> args |> List.map (fun (t, _) -> term_to_string opts t) |> String.concat "; ") |> String.concat "\/" in
         U.format1 "{Meta_pattern %s}" pats
 
     | Meta_named lid ->
-        U.format1 "{Meta_named %s}" (sli lid)
+        U.format1 "{Meta_named %s}" (sli opts lid)
 
     | Meta_labeled (l, r, _) ->
         U.format2 "{Meta_labeled (%s, %s)}" l (Range.string_of_range r)
@@ -600,38 +600,38 @@ and metadata_to_string = function
         "{Meta_desugared}"
 
     | Meta_monadic (m, t) ->
-        U.format2 "{Meta_monadic(%s @ %s)}" (sli m) (term_to_string t)
+        U.format2 "{Meta_monadic(%s @ %s)}" (sli opts m) (term_to_string opts t)
 
     | Meta_monadic_lift (m, m', t) ->
-        U.format3 "{Meta_monadic_lift(%s -> %s @ %s)}" (sli m) (sli m') (term_to_string t)
+        U.format3 "{Meta_monadic_lift(%s -> %s @ %s)}" (sli opts m) (sli opts m') (term_to_string opts t)
 
 let aqual_to_string aq = aqual_to_string' "" aq
-let bqual_to_string bq = bqual_to_string' "" bq
+let bqual_to_string opts bq = bqual_to_string' opts "" bq
 
-let comp_to_string' env c =
-  if Options.ugly ()
-  then comp_to_string c
+let comp_to_string' opts env c =
+  if opts.ugly
+  then comp_to_string opts c
   else let e = Resugar.resugar_comp' env c in
        let d = ToDocument.term_to_document e in
        Pp.pretty_string (float_of_string "1.0") 100 d
 
-let term_to_string' env x =
-  if Options.ugly ()
-  then term_to_string x
+let term_to_string' opts env x =
+  if opts.ugly
+  then term_to_string opts x
   else let e = Resugar.resugar_term' env x in
        let d = ToDocument.term_to_document e in
        Pp.pretty_string (float_of_string "1.0") 100 d
 
-let binder_to_json env b =
-    let n = JsonStr (bqual_to_string' (nm_to_string b.binder_bv) b.binder_qual) in
-    let t = JsonStr (term_to_string' env b.binder_bv.sort) in
+let binder_to_json opts env b =
+    let n = JsonStr (bqual_to_string' opts (nm_to_string opts b.binder_bv) b.binder_qual) in
+    let t = JsonStr (term_to_string' opts env b.binder_bv.sort) in
     JsonAssoc [("name", n); ("type", t)]
 
-let binders_to_json env bs =
-    JsonList (List.map (binder_to_json env) bs)
+let binders_to_json opts env bs =
+    JsonList (List.map (binder_to_json opts env) bs)
 
 
-//let subst_to_string subst =
+//let subst_to_string opts subst =
 //   U.format1 "{%s}" <|
 //    (List.map (function
 //        | Inl (a, t) -> U.format2 "(%s -> %s)" (strBvd a) (typ_to_string t)
@@ -641,31 +641,31 @@ let binders_to_json env bs =
 //    U.format2 "ftvs={%s}, fxvs={%s}" (f fvs.ftvs) (f fvs.fxvs)
 
 
-let enclose_universes s =
-    if Options.print_universes ()
+let enclose_universes opts s =
+    if opts.print_universes
     then "<" ^ s ^ ">"
     else ""
 
-let tscheme_to_string s =
-  if not (Options.ugly()) then
+let tscheme_to_string opts s =
+  if not opts.ugly then
     let d = Resugar.resugar_tscheme s in
     let d = ToDocument.decl_to_document d in
     Pp.pretty_string (float_of_string "1.0") 100 d
   else
     let (us, t) = s in
-    U.format2 "%s%s" (enclose_universes <| univ_names_to_string us) (term_to_string t)
+    U.format2 "%s%s" (enclose_universes opts <| univ_names_to_string us) (term_to_string opts t)
 
-let action_to_string a =
+let action_to_string opts a =
     U.format5 "%s%s %s : %s = %s"
-        (sli a.action_name)
-        (binders_to_string " " a.action_params)
-        (enclose_universes <| univ_names_to_string a.action_univs)
-        (term_to_string a.action_typ)
-        (term_to_string a.action_defn)
+        (sli opts a.action_name)
+        (binders_to_string opts " " a.action_params)
+        (enclose_universes opts <| univ_names_to_string a.action_univs)
+        (term_to_string opts a.action_typ)
+        (term_to_string opts a.action_defn)
 
-let wp_eff_combinators_to_string combs =
+let wp_eff_combinators_to_string opts combs =
   let tscheme_opt_to_string = function
-    | Some ts -> tscheme_to_string ts
+    | Some ts -> tscheme_to_string opts ts
     | None -> "None" in
 
   U.format "{\n\
@@ -680,21 +680,21 @@ let wp_eff_combinators_to_string combs =
   ; return_repr  = %s\n\
   ; bind_repr    = %s\n\
   }\n"
-    [ tscheme_to_string combs.ret_wp;
-      tscheme_to_string combs.bind_wp;
-      tscheme_to_string combs.stronger;
-      tscheme_to_string combs.if_then_else;
-      tscheme_to_string combs.ite_wp;
-      tscheme_to_string combs.close_wp;
-      tscheme_to_string combs.trivial;
+    [ tscheme_to_string opts combs.ret_wp;
+      tscheme_to_string opts combs.bind_wp;
+      tscheme_to_string opts combs.stronger;
+      tscheme_to_string opts combs.if_then_else;
+      tscheme_to_string opts combs.ite_wp;
+      tscheme_to_string opts combs.close_wp;
+      tscheme_to_string opts combs.trivial;
       tscheme_opt_to_string combs.repr;
       tscheme_opt_to_string combs.return_repr;
       tscheme_opt_to_string combs.bind_repr ]
 
-let layered_eff_combinators_to_string combs =
+let layered_eff_combinators_to_string opts combs =
   let to_str (ts_t, ts_ty) =
     U.format2 "(%s) : (%s)"
-      (tscheme_to_string ts_t) (tscheme_to_string ts_ty) in
+      (tscheme_to_string opts ts_t) (tscheme_to_string opts ts_ty) in
 
   U.format "{\n\
   ; l_repr = %s\n\
@@ -709,20 +709,20 @@ let layered_eff_combinators_to_string combs =
       to_str combs.l_subcomp;
       to_str combs.l_if_then_else ]
 
-let eff_combinators_to_string = function
+let eff_combinators_to_string opts = function
   | Primitive_eff combs
-  | DM4F_eff combs -> wp_eff_combinators_to_string combs
-  | Layered_eff combs -> layered_eff_combinators_to_string combs
+  | DM4F_eff combs -> wp_eff_combinators_to_string opts combs
+  | Layered_eff combs -> layered_eff_combinators_to_string opts combs
 
-let eff_decl_to_string' for_free r q ed =
- if not (Options.ugly()) then
+let eff_decl_to_string' opts for_free r q ed =
+ if not opts.ugly then
     let d = Resugar.resugar_eff_decl r q ed in
     let d = ToDocument.decl_to_document d in
     Pp.pretty_string (float_of_string "1.0") 100 d
  else
     let actions_to_string actions =
         actions |>
-        List.map action_to_string |>
+        List.map (action_to_string opts) |>
         String.concat ",\n\t" in
     let eff_name = if SU.is_layered ed then "layered_effect" else "new_effect" in
     U.format "%s%s { \
@@ -731,22 +731,22 @@ let eff_decl_to_string' for_free r q ed =
       and effect_actions\n\t%s\n}\n"
         [eff_name;
          (if for_free then "_for_free " else "");
-         lid_to_string ed.mname;
-         enclose_universes <| univ_names_to_string ed.univs;
-         binders_to_string " " ed.binders;
-         tscheme_to_string ed.signature;
-         eff_combinators_to_string ed.combinators;
+         lid_to_string opts ed.mname;
+         enclose_universes opts <| univ_names_to_string ed.univs;
+         binders_to_string opts " " ed.binders;
+         tscheme_to_string opts ed.signature;
+         eff_combinators_to_string opts ed.combinators;
          actions_to_string ed.actions]
 
-let eff_decl_to_string for_free ed =
-  eff_decl_to_string' for_free Range.dummyRange [] ed
+let eff_decl_to_string opts for_free ed =
+  eff_decl_to_string' opts for_free Range.dummyRange [] ed
 
-let sub_eff_to_string se =
+let sub_eff_to_string opts se =
   let tsopt_to_string ts_opt =
-    if is_some ts_opt then ts_opt |> must |> tscheme_to_string
+    if is_some ts_opt then ts_opt |> must |> tscheme_to_string opts
     else "<None>" in
   U.format4 "sub_effect %s ~> %s : lift = %s ;; lift_wp = %s"
-    (lid_to_string se.source) (lid_to_string se.target)
+    (lid_to_string opts se.source) (lid_to_string opts se.target)
     (tsopt_to_string se.lift) (tsopt_to_string se.lift_wp)
 
 let pragma_to_string (p:pragma) : string =
@@ -760,8 +760,8 @@ let pragma_to_string (p:pragma) : string =
   | PrintEffectsGraph     -> "#print-effects-graph"
   | PopOptions            -> "#pop-options"
 
-let rec sigelt_to_string (x: sigelt) =
- // if not (Options.ugly()) then
+let rec sigelt_to_string opts (x: sigelt) =
+ // if not (opts.ugly()) then
  //    let e = Resugar.resugar_sigelt x in
  //    begin match e with
  //    | Some d ->
@@ -774,80 +774,80 @@ let rec sigelt_to_string (x: sigelt) =
       match x.sigel with
       | Sig_pragma p -> pragma_to_string p
       | Sig_inductive_typ(lid, univs, tps, k, _, _) ->
-        let quals_str = quals_to_string' x.sigquals in
-        let binders_str = binders_to_string " " tps in
-        let term_str = term_to_string k in
-        if Options.print_universes () then U.format5 "%stype %s<%s> %s : %s" quals_str (string_of_lid lid) (univ_names_to_string univs) binders_str term_str
+        let quals_str = quals_to_string' opts  x.sigquals in
+        let binders_str = binders_to_string opts " " tps in
+        let term_str = term_to_string opts k in
+        if opts.print_universes then U.format5 "%stype %s<%s> %s : %s" quals_str (string_of_lid lid) (univ_names_to_string univs) binders_str term_str
         else U.format4 "%stype %s %s : %s" quals_str (string_of_lid lid) binders_str term_str
       | Sig_datacon(lid, univs, t, _, _, _) ->
-        if (Options.print_universes())
+        if opts.print_universes
         then //let univs, t = Subst.open_univ_vars univs t in (* AR: don't open the universes, else it's a bit confusing *)
-             U.format3 "datacon<%s> %s : %s" (univ_names_to_string univs) (string_of_lid lid) (term_to_string t)
-        else U.format2 "datacon %s : %s" (string_of_lid lid) (term_to_string t)
+             U.format3 "datacon<%s> %s : %s" (univ_names_to_string univs) (string_of_lid lid) (term_to_string opts t)
+        else U.format2 "datacon %s : %s" (string_of_lid lid) (term_to_string opts t)
       | Sig_declare_typ(lid, univs, t) ->
         //let univs, t = Subst.open_univ_vars univs t in
-        U.format4 "%sval %s %s : %s" (quals_to_string' x.sigquals) (string_of_lid lid)
-            (if (Options.print_universes())
+        U.format4 "%sval %s %s : %s" (quals_to_string' opts  x.sigquals) (string_of_lid lid)
+            (if opts.print_universes
              then U.format1 "<%s>" (univ_names_to_string univs)
              else "")
-            (term_to_string t)
+            (term_to_string opts t)
       | Sig_assume(lid, us, f) ->
-        if Options.print_universes () then U.format3 "assume %s<%s> : %s" (string_of_lid lid) (univ_names_to_string us) (term_to_string f)
-        else U.format2 "assume %s : %s" (string_of_lid lid) (term_to_string f)
-      | Sig_let(lbs, _) -> lbs_to_string x.sigquals lbs
-      | Sig_bundle(ses, _) -> "(* Sig_bundle *)" ^ (List.map sigelt_to_string ses |> String.concat "\n")
+        if opts.print_universes then U.format3 "assume %s<%s> : %s" (string_of_lid lid) (univ_names_to_string us) (term_to_string opts f)
+        else U.format2 "assume %s : %s" (string_of_lid lid) (term_to_string opts f)
+      | Sig_let(lbs, _) -> lbs_to_string opts x.sigquals lbs
+      | Sig_bundle(ses, _) -> "(* Sig_bundle *)" ^ (List.map (sigelt_to_string opts) ses |> String.concat "\n")
       | Sig_fail (errs, lax, ses) ->
         U.format3 "(* Sig_fail %s %s *)\n%s\n(* / Sig_fail*)\n"
             (string_of_bool lax)
             (FStar.Common.string_of_list string_of_int errs)
-            (List.map sigelt_to_string ses |> String.concat "\n")
+            (List.map (sigelt_to_string opts) ses |> String.concat "\n")
 
-      | Sig_new_effect(ed) -> eff_decl_to_string' (SU.is_dm4f ed) x.sigrng x.sigquals ed
-      | Sig_sub_effect (se) -> sub_eff_to_string se
+      | Sig_new_effect(ed) -> eff_decl_to_string' opts (SU.is_dm4f ed) x.sigrng x.sigquals ed
+      | Sig_sub_effect (se) -> sub_eff_to_string opts se
       | Sig_effect_abbrev(l, univs, tps, c, flags) ->
-        if (Options.print_universes())
+        if opts.print_universes
         then let univs, t = Subst.open_univ_vars univs (mk (Tm_arrow(tps, c)) Range.dummyRange) in
              let tps, c = match (Subst.compress t).n with
                 | Tm_arrow(bs, c) -> bs, c
                 | _ -> failwith "impossible" in
-             U.format4 "effect %s<%s> %s = %s" (sli l) (univ_names_to_string univs) (binders_to_string " " tps) (comp_to_string c)
-        else U.format3 "effect %s %s = %s" (sli l) (binders_to_string " " tps) (comp_to_string c)
+             U.format4 "effect %s<%s> %s = %s" (sli opts l) (univ_names_to_string univs) (binders_to_string opts " " tps) (comp_to_string opts c)
+        else U.format3 "effect %s %s = %s" (sli opts l) (binders_to_string opts " " tps) (comp_to_string opts c)
       | Sig_splice (lids, t) ->
-        U.format2 "splice[%s] (%s)" (String.concat "; " <| List.map Ident.string_of_lid lids) (term_to_string t)
+        U.format2 "splice[%s] (%s)" (String.concat "; " <| List.map Ident.string_of_lid lids) (term_to_string opts t)
       | Sig_polymonadic_bind (m, n, p, t, ty) ->
         U.format5 "polymonadic_bind (%s, %s) |> %s = (%s, %s)"
           (Ident.string_of_lid m)
           (Ident.string_of_lid n)
           (Ident.string_of_lid p)
-          (tscheme_to_string t)
-          (tscheme_to_string ty)
+          (tscheme_to_string opts t)
+          (tscheme_to_string opts ty)
       | Sig_polymonadic_subcomp (m, n, t, ty) ->
         U.format4 "polymonadic_subcomp %s <: %s = (%s, %s)"
           (Ident.string_of_lid m)
           (Ident.string_of_lid n)
-          (tscheme_to_string t)
-          (tscheme_to_string ty)
+          (tscheme_to_string opts t)
+          (tscheme_to_string opts ty)
       in
       match x.sigattrs with
       | [] -> "[@ ]" ^ "\n" ^ basic //It is important to keep this empty attribute marker since the Vale type extractor uses it as a delimiter
-      | _ -> attrs_to_string x.sigattrs ^ "\n" ^ basic
+      | _ -> attrs_to_string opts x.sigattrs ^ "\n" ^ basic
 
 (* A "short" version of printing a sigelt. Meant to (usually) be a small string
 suitable to embed in an error message. No need to be fully faithful to
 printing universes, etc, it should just make it clear enough to which
 sigelt it refers to. *)
-let rec sigelt_to_string_short (x: sigelt) = match x.sigel with
+let rec sigelt_to_string_short opts (x: sigelt) = match x.sigel with
   | Sig_pragma p ->
     pragma_to_string p
 
   | Sig_let((false, [{lbname=lb}]), _) ->
-    U.format1 "let %s" (lbname_to_string lb)
+    U.format1 "let %s" (lbname_to_string opts lb)
 
   | Sig_let((true, [{lbname=lb}]), _) ->
-    U.format1 "let rec %s" (lbname_to_string lb)
+    U.format1 "let rec %s" (lbname_to_string opts lb)
 
   | Sig_let((true, ({lbname=lb})::_), _) ->
-    U.format1 "let rec %s and ..." (lbname_to_string lb)
+    U.format1 "let rec %s and ..." (lbname_to_string opts lb)
 
   | Sig_let _ ->
     failwith "Impossible: sigelt_to_string_short, ill-formed let"
@@ -859,15 +859,15 @@ let rec sigelt_to_string_short (x: sigelt) = match x.sigel with
     U.format1 "type %s" (string_of_lid lid)
 
   | Sig_datacon(lid, _, t, _, _, _) ->
-    U.format2 "datacon %s : %s" (string_of_lid lid) (term_to_string t)
+    U.format2 "datacon %s : %s" (string_of_lid lid) (term_to_string opts t)
 
   | Sig_assume(lid, us, f) ->
-    U.format2 "assume %s : %s" (string_of_lid lid) (term_to_string f)
+    U.format2 "assume %s : %s" (string_of_lid lid) (term_to_string opts f)
 
-  | Sig_bundle(ses, _) -> List.hd ses |> sigelt_to_string_short
+  | Sig_bundle(ses, _) -> List.hd ses |> sigelt_to_string_short opts
 
   | Sig_fail (errs, lax, ses) ->
-    U.format1 "[@@expect_failure] %s" (ses |> List.hd |> sigelt_to_string_short)
+    U.format1 "[@@expect_failure] %s" (ses |> List.hd |> sigelt_to_string_short opts)
 
   | Sig_new_effect ed ->
     let kw =
@@ -875,19 +875,19 @@ let rec sigelt_to_string_short (x: sigelt) = match x.sigel with
       else if SU.is_dm4f ed then "new_effect_for_free"
       else "new_effect"
     in
-    U.format2 "%s { %s ... }" kw (lid_to_string ed.mname)
+    U.format2 "%s { %s ... }" kw (lid_to_string opts ed.mname)
 
   | Sig_sub_effect se ->
-    U.format2 "sub_effect %s ~> %s" (lid_to_string se.source) (lid_to_string se.target)
+    U.format2 "sub_effect %s ~> %s" (lid_to_string opts se.source) (lid_to_string opts se.target)
 
   | Sig_effect_abbrev (l, univs, tps, c, flags) ->
-    U.format3 "effect %s %s = %s" (sli l) (binders_to_string " " tps) (comp_to_string c)
+    U.format3 "effect %s %s = %s" (sli opts l) (binders_to_string opts " " tps) (comp_to_string opts c)
 
   | Sig_splice (lids, t) ->
     U.format3 "%splice[%s] (%s)"
               "%s" // sigh, no escape for format
               (String.concat "; " <| List.map Ident.string_of_lid lids)
-              (term_to_string t)
+              (term_to_string opts t)
 
   | Sig_polymonadic_bind (m, n, p, t, ty) ->
     U.format3 "polymonadic_bind (%s, %s) |> %s"
@@ -896,7 +896,7 @@ let rec sigelt_to_string_short (x: sigelt) = match x.sigel with
   | Sig_polymonadic_subcomp (m, n, t, ty) ->
     U.format2 "polymonadic_subcomp %s <: %s" (Ident.string_of_lid m) (Ident.string_of_lid n)
 
-let tag_of_sigelt (se:sigelt) : string =
+let tag_of_sigelt opts (se:sigelt) : string =
   match se.sigel with
   | Sig_inductive_typ _    -> "Sig_inductive_typ"
   | Sig_bundle _           -> "Sig_bundle"
@@ -916,10 +916,10 @@ let tag_of_sigelt (se:sigelt) : string =
 (*
  * AR: 07/19: exports is redundant, keeping it here until vale is fixed to not parse it
  *)
-let modul_to_string (m:modul) =
-  U.format3 "module %s\nDeclarations: [\n%s\n]\nExports: [\n%s\n]\n" (sli m.name)
-                                                                     (List.map sigelt_to_string m.declarations |> String.concat "\n")
-                                                                     (List.map sigelt_to_string m.declarations |> String.concat "\n")
+let modul_to_string opts (m:modul) =
+  U.format3 "module %s\nDeclarations: [\n%s\n]\nExports: [\n%s\n]\n" (sli opts m.name)
+                                                                     (List.map (sigelt_to_string opts) m.declarations |> String.concat "\n")
+                                                                     (List.map (sigelt_to_string opts) m.declarations |> String.concat "\n")
 
 
 //let abs_ascription_to_string ascription =
@@ -935,7 +935,7 @@ let modul_to_string (m:modul) =
 //  end ;
 //  U.string_of_string_builder strb
 
-let list_to_string f elts =
+let list_to_string opts f elts =
     match elts with
         | [] -> "[]"
         | x::xs ->
@@ -949,7 +949,7 @@ let list_to_string f elts =
             U.string_builder_append strb "]" ;
             U.string_of_string_builder strb
 
-let set_to_string f s =
+let set_to_string opts f s =
     let elts = U.set_elements s in
     match elts with
         | [] -> "{}"
@@ -962,17 +962,17 @@ let set_to_string f s =
                        U.string_builder_append strb (f x)
                        ) xs ;
             U.string_builder_append strb "}" ;
-            (* U.string_builder_append strb (list_to_string f (raw_list s)) ; *)
+            (* U.string_builder_append strb (list_to_string opts f (raw_list s)) ; *)
             U.string_of_string_builder strb
 
-let bvs_to_string sep bvs = binders_to_string sep (List.map mk_binder bvs)
+let bvs_to_string opts sep bvs = binders_to_string opts sep (List.map mk_binder bvs)
 
-let ctx_uvar_to_string ctx_uvar = ctx_uvar_to_string_aux true ctx_uvar
+let ctx_uvar_to_string opts ctx_uvar = ctx_uvar_to_string_aux opts true ctx_uvar
 
-let ctx_uvar_to_string_no_reason ctx_uvar = ctx_uvar_to_string_aux false ctx_uvar
+let ctx_uvar_to_string_no_reason opts ctx_uvar = ctx_uvar_to_string_aux opts false ctx_uvar
 
-let rec emb_typ_to_string = function
+let rec emb_typ_to_string opts = function
     | ET_abstract -> "abstract"
     | ET_app (h, []) -> h
-    | ET_app(h, args) -> "(" ^h^ " " ^ (List.map emb_typ_to_string args |> String.concat " ")  ^")"
-    | ET_fun(a, b) -> "(" ^ emb_typ_to_string a ^ ") -> " ^ emb_typ_to_string b
+    | ET_app(h, args) -> "(" ^h^ " " ^ (List.map (emb_typ_to_string opts) args |> String.concat " ")  ^")"
+    | ET_fun(a, b) -> "(" ^ emb_typ_to_string opts a ^ ") -> " ^ emb_typ_to_string opts b
